single_invocation_correctness.thy
@@ -28,7 +28,7 @@ definition initialStates :: "('localState, 'any) prog \<Rightarrow> ('localState
 
 (* check program (with a given start-state, bound by a number of steps) *)
 fun checkCorrect :: "('localState, 'any) prog \<Rightarrow> ('localState, 'any) state \<Rightarrow> invocation \<Rightarrow> nat \<Rightarrow> bool" where
-"checkCorrect progr S i 0 = False"
+"checkCorrect progr S i 0 = True"
 | "checkCorrect progr S i (Suc bound) =
 (case currentProc S i of
     None \<Rightarrow> True
@@ -95,6 +95,147 @@ fun checkCorrect :: "('localState, 'any) prog \<Rightarrow> ('localState, 'any) 
         ))
 "
 
+
+lemma prog_invariant:
+assumes steps: "S_start ~~ (i, trace) \<leadsto>\<^sub>S* S_fin"
+shows "prog S_fin = prog S_start"
+using steps proof (induct rule: step_s_induct)
+  case initial
+  then show ?case by auto
+next
+  case (step tr S a S')
+  then show ?case 
+    by (auto simp add: step_s.simps)
+qed
+
+
+lemma 
+assumes check: "checkCorrect program S_start i bound"
+    and steps: "S_start ~~ (i, trace) \<leadsto>\<^sub>S* S_fin"
+    and trace_len: "length trace < bound"
+    and prog: "prog S_start = program"
+    and noInvocation: "\<And>a c. (a,c)\<in>set trace \<Longrightarrow> \<not> isAInvoc a"
+shows "traceCorrect_s program trace \<and> checkCorrect program S_fin i (bound - length trace)"
+using steps check trace_len noInvocation proof (induct "length trace" arbitrary: S_fin trace)
+  case 0
+  hence [simp]: "trace = []" by simp
+  with `S_start ~~ (i, trace) \<leadsto>\<^sub>S* S_fin` 
+  have [simp]: "S_fin = S_start"
+    by (simp add: steps_s_empty) 
+ 
+  from `checkCorrect program S_start i bound` 
+  show ?case
+    by (auto simp add: traceCorrect_s_def )
+next
+  case (Suc n)
+  
+  from `Suc n = length trace`
+  obtain tr a where trace_split: "trace = tr@[a]"
+    by (metis Zero_not_Suc list.size(3) rev_exhaust)
+   
+  with `S_start ~~ (i, trace) \<leadsto>\<^sub>S* S_fin`  
+  obtain S where steps_tr: "S_start ~~ (i, tr) \<leadsto>\<^sub>S* S" and step_a: "S ~~ (i, a) \<leadsto>\<^sub>S S_fin"
+    using steps_s_append_simp steps_s_single by blast
+    
+    
+  have IH: "traceCorrect_s program tr \<and> checkCorrect program S i (bound - length tr)"
+  proof (rule Suc.hyps)
+    show "n = length tr"
+      using Suc.hyps(2) trace_split by auto
+    show "S_start ~~ (i, tr) \<leadsto>\<^sub>S* S" using steps_tr .
+    show "checkCorrect program S_start i bound" using `checkCorrect program S_start i bound` .
+    show "length tr < bound"
+      using Suc.hyps(2) Suc.prems(3) \<open>n = length tr\<close> by linarith 
+    show "\<And>a c. (a, c) \<in> set tr \<Longrightarrow> \<not> isAInvoc a"
+      using Suc.prems(4) trace_split by auto
+  qed
+  hence "traceCorrect_s program tr" and "checkCorrect program S i (bound - length tr)" by auto
+  
+  obtain bound' where bound'_def: "bound - length tr = Suc bound'"
+    by (metis Suc.prems(3) Suc_diff_Suc Suc_lessD length_append_singleton trace_split) 
+    
+  hence checkCorrect_S: "checkCorrect program S i (Suc bound')"
+    using `checkCorrect program S i (bound - length tr)` by simp
+  
+  have [simp]: "bound - length trace = bound'"
+    by (metis Suc_diff_Suc Suc_inject bound'_def length_append_singleton trace_split zero_less_Suc zero_less_diff)  
+   
+  have [simp]: "prog S = program"
+    using prog prog_invariant steps_tr by blast
+    
+  have a_not_invoc: "\<not> isAInvoc (fst a)"
+    by (metis Suc.prems(4) list.set_intros(1) prod.collapse rotate1.simps(2) set_rotate1 trace_split)
+    
+    
+  from step_a
+  have "snd a \<and> checkCorrect program S_fin i (bound - length trace)" 
+  proof (cases rule: step_s.cases)
+    case (local ls f ls')
+    then show ?thesis 
+      using checkCorrect_S by auto
+      
+    
+  next
+    case (newId ls f ls' uid)
+    then show ?thesis using checkCorrect_S by auto
+  next
+    case (beginAtomic ls f ls' t txns)
+    then show ?thesis 
+      using checkCorrect_S apply auto
+      using local.beginAtomic(13) by blast
+  next
+    case (endAtomic ls f ls' t valid)
+    then show ?thesis using checkCorrect_S by auto
+  next
+    case (dbop ls f Op args ls' t c res vis)
+    then show ?thesis 
+      using checkCorrect_S by auto
+  next
+    case (invocation procName args initState impl C' valid)
+    then show ?thesis 
+      using a_not_invoc by (case_tac a, auto simp add: isAInvoc_def)
+  next
+    case (return ls f res valid)
+    then show ?thesis using checkCorrect_S 
+    by (case_tac bound', auto)
+  qed
+  thus "traceCorrect_s program trace \<and> checkCorrect program S_fin i (bound - length trace)"
+    apply auto
+    by (metis IH Pair_inject Un_insert_right append_Nil2 insert_iff list.set(2) prod.collapse set_append traceCorrect_s_def trace_split)
+  
+qed  
+    
+(*
+now we have it without invocations, so we have to prove that invocations can only be at the beginning, then we are in initial states ...
+*)
+
+lemma 
+assumes initialCorrect: "\<And>S. S\<in>initialStates program \<Longrightarrow> invariant_all S "
+    and check: "\<And>S i. S\<in>initialStates program \<Longrightarrow> checkCorrect program S i bound"
+    and steps: "initialState program ~~ (i, trace) \<leadsto>\<^sub>S* S_fin"
+    and trace_len: "length trace < bound"
+    and trace_len2: "0 < length trace"
+shows "traceCorrect_s program trace \<and> checkCorrect program S_fin i (bound - length trace)"
+using steps check trace_len proof (induct "length trace")
+  case 0
+  thus ?case
+    using trace_len2 by linarith 
+    
+next
+  case (Suc trLen)
+  
+  
+  
+  obtain tr a where tr_def: "trace = tr@[a]"
+    
+  
+  
+  then show ?case sorry
+qed
+
+
+
+    
 lemma show_program_correct_single_invocation:
 assumes initialCorrect: "\<And>S. S\<in>initialStates program \<Longrightarrow> invariant_all S "
     and check: "\<And>S i. S\<in>initialStates program \<Longrightarrow> checkCorrect program S i bound"
